\renewcommand{\arraystretch}{1.25}
\begin{tabularx}{\textwidth}{|@{}r@{\hspace{2pt}}X@{}|}
	\hline
	% derivation of product
	\(\sM^0_{2}\) & \( = \displaystyle
	m^0_1 \circ_1 m^0_2
	- m^0_2 \circ_1 m^0_1
	- m^0_2 \circ_2 m^0_1
	= [m^0_1, m^0_2] \) \\

	\hline
	% commutativity of differential and codifferential
	\(\sM^1_1\) & \( = \displaystyle m^0_1 \circ m^1_1 + m^1_1 \circ m^0_1 \)
	\( = [m^0_1, m^1_1] \) \\

	\hline
	% derivation of the bracket
	\(\sM^0_{1,1}\) & \( = \displaystyle
	m^0_1 \circ m^0_{1,1}
	- m^0_{1,1} \circ_1 m^0_1
	- m^0_{1,1} \circ_2 m^0_1
	= [m^0_1, m^0_{1,1}] \) \\

	\hline
\end{tabularx}
